\begin{frame}{\mytitle{What about laws of conservation?}}
$$(\mathbbm{H}\mathbbm{S}^{-1}\boldsymbol{\tau})_{mk}=\sum_{n,r=1}^N\mathbbm{H}_{mn}\mathbbm{S}^{-1}_{nr}\boldsymbol{\tau}_{rk}=$$
$$=\sum_{n,r=1}^N\mymean{\phi_m}{\hat{H}}{\phi_n}\mathbbm{S}^{-1}_{nr}\sum_{l=1}^M\myelr{\phi_r}{\frac{\partial\phi_k}{\partial\lambda_{kl}}}\dot{\lambda}_{kl}=$$
$$=\sum_{l=1}^M\mymean{\phi_m}{\hat{H}\left(\sum_{n,r=1}^N|\phi_n\rangle\mathbbm{S}^{-1}_{nr}\langle\phi_r|\right)}{\frac{\partial\phi_k}{\partial\lambda_{kl}}}\dot{\lambda}_{kl}=%
\sum_{l=1}^M\mymean{\phi_m}{\hat{H}\hat{P}}{\frac{\partial\phi_k}{\partial\lambda_{kl}}}\dot{\lambda}_{kl}$$
$$(\dot{\mathbbm{H}} - \mathbbm{H}\mathbbm{S}^{-1}\boldsymbol{\tau}-\boldsymbol{\tau}^{\dagger}\mathbbm{S}^{-1}\mathbbm{H})_{mk}=$$
$$=\sum_{l=1}^M\mymean{\phi_m}%
		      {\hat{H}(\hat{1}-\hat{P})}%
		      {\frac{\partial\phi_k}{\partial\lambda_{kl}}}\dot{\lambda}_{kl}+%
	       \mymean{\frac{\partial\phi_m}{\partial\lambda_{ml}}}%
		      {(\hat{1}-\hat{P})\hat{H}}%
		      {\phi_k}\dot{\lambda}_{ml}^*\neq0$$

\end{frame}

