Let us assume, that function $|\Psi\rangle$ can be spanned over linear combination of basis functions $\{|\phi_k(\vec{\lambda})\rangle\}_{k=1}^N$:
$$|\Psi\rangle = \sum_{k=1}^NC_k(t)|\phi_k(\vec{\lambda})\rangle, \dim\{\vec{\lambda}\} = M$$
Then we can consider a variation of $|\Psi\rangle$:
$$|\delta\Psi\rangle = \sum_{k=1}^N \left( \delta C_k|\phi_k\rangle + %
					   C_k\sum_{j=1}^M|\frac{\partial\phi_k}{\partial\lambda_{kj}}\rangle\delta\lambda_{kj} \right)$$
Thus, using Dirac--Frenkel variational principle, we will obtain:
$$\delta C_m^*\sum_{k=1}^N\langle\phi_m|\hat{H}-i\hbar\frac{\partial}{\partial t}|C_k\phi_k\rangle=0$$
$$\delta\lambda_{mj}^*\sum_{k=0}^NC_m^*\langle\frac{\partial\phi_m}{\partial\lambda_{mj}}|\hat{H}-i\hbar\frac{\partial}{\partial t}|C_k\phi_k\rangle = 0$$
As variations are independant and arbitrary, we will get two sets of equations:
$$\sum_{k=1}^N\langle\phi_m|\hat{H}-i\hbar\frac{\partial}{\partial t}|C_k\phi_k\rangle=0$$
$$\sum_{k=0}^NC_m^*\langle\frac{\partial\phi_m}{\partial\lambda_{mj}}|\hat{H}-i\hbar\frac{\partial}{\partial t}|C_k\phi_k\rangle = 0$$

Let us consider the first equation:
$$\sum_{k=1}^N C_k\langle\phi_m|\hat{H}|\phi_k\rangle - %
	       i\hbar\langle\phi_m|\phi_k\rangle \dot{C}_k - %
	       i\hbar\sum_{l=1}^M\langle\phi_m|\frac{\partial\phi_k}{\partial\lambda_{kl}}\rangle\dot{\lambda}_{kl}=0$$
$$i\hbar\sum_{k=1}^N\mathbbm{S}_{mk}\dot{C}_k=\sum_{k=1}^N\left(\mathbbm{H}_{mk}-%
							  i\hbar\sum_{l=1}^M\langle\phi_m|\frac{\partial\phi_k}{\partial\lambda_{kl}}\rangle\dot{\lambda}_{kl}\right)C_k$$
$$i\hbar\mathbbm{S}\dot{\vec{C}}=(\mathbbm{H}-i\hbar\tau)\vec{C}$$
$$\dot{\vec{C}} = -\frac{i}{\hbar}\mathbbm{S}^{-1}(\mathbbm{H}-i\hbar\tau)\vec{C}$$
$$\dot{C}_k = -\frac{i}{\hbar}\sum_{n,r=1}^N \mathbbm{S}^{-1}_{kn}(\mathbbm{H}_{nr}-i\hbar\tau_{nr})C_r$$
And the second one:
$$\sum_{k=1}^N\left(C_m^*C_k\langle\frac{\partial\phi_m}{\partial\lambda_{mj}}|\hat{H}|\phi_k\rangle-%
	     i\hbar\langle\frac{\partial\phi_m}{\partial\lambda_{mj}}|\phi_k\rangle C_m^*\dot{C}_k-%
	     i\hbar\sum_{l=1}^MC_m^*C_k\langle\frac{\partial\phi_m}{\partial\lambda_{mj}}|\frac{\partial\phi_k}{\partial\lambda_{kl}}\rangle\dot{\lambda}_{kl}\right)=0$$
$$\sum_{k=1}^N\left(C_m^*C_k\langle\frac{\partial\phi_m}{\partial\lambda_{mj}}|\hat{H}|\phi_k\rangle-%
		    \langle\frac{\partial\phi_m}{\partial\lambda_{mj}}|\phi_k\rangle\sum_{n,r=1}^N\mathbbm{S}^{-1}_{kn}\mathbbm{H}_{nr}C_m^*C_r\right)=$$
$$= \sum_{k=1}^N\left(-i\hbar\sum_{n,r=1}^N\langle\frac{\partial\phi_m}{\partial\lambda_{mj}}|\phi_k\rangle\mathbbm{S}_{kn}^{-1}%
		             \sum_{l=1}^M\langle\phi_n|\frac{\partial\phi_r}{\partial\lambda_{rl}}\rangle\dot{\lambda}_{rl}C_m^*C_r+%
     		       i\hbar\sum_{l=1}^MC_m^*C_k\langle\frac{\partial\phi_m}{\partial\lambda_{mj}}|\frac{\partial\phi_k}{\partial\lambda_{kl}}\rangle\dot{\lambda}_{kl}\right)$$

$$\rho_{mk} = C_m^*C_k$$
$$\mathbbm{H}_{ml}^{(j0)}=\langle\frac{\partial\phi_m}{\partial\lambda_{mj}}|\hat{H}|\phi_k\rangle$$
$$\mathbbm{S}_{mk}^{(j0)}=\langle\frac{\partial\phi_m}{\partial\lambda_{mj}}|\phi_k\rangle$$
$$\mathbbm{S}_{nr}^{(0l)}=\langle\phi_n|\frac{\partial\phi_r}{\partial\lambda_{rl}}\rangle$$
$$\mathbbm{S}_{mk}^{(jl)}=\langle\frac{\partial\phi_m}{\partial\lambda_{mj}}|%
				 \frac{\partial\phi_k}{\partial\lambda_{kl}}\rangle$$
$$\sum_{k=1}^N\rho_{mk}\mathbbm{H}_{mk}^{(j0)}-%
  \sum_{r=1}^N\rho_{mr}\left(\sum_{k,n=1}^N\mathbbm{S}_{mk}^{(j0)}\mathbbm{S}_{kn}^{-1}\mathbbm{H}_{nr}\right)=$$
$$=i\hbar\sum_{l=1}^M\left(\sum_{k=1}^N\rho_{mk}\mathbbm{S}_{mk}^{(jl)}\dot{\lambda}_{kl}-%
\sum_{r=1}^N\rho_{mr}\left(\sum_{k,n=1}^{N}\mathbbm{S}_{mk}^{(j0)}\mathbbm{S}_{kn}^{-1}\mathbbm{S}_{nr}^{(0l)}\right)\dot{\lambda}_{rl}\right)$$
$$\sum_{k=1}^N\rho_{mk}\left(\mathbbm{H}_{mk}^{(j0)}-%
	                     (\mathbbm{S}^{(j0)}\mathbbm{S}^{-1}\mathbbm{H})_{mk} \right)=%
i\hbar\sum_{l=1}^M\sum_{k=1}^N\rho_{mk}\left(\mathbbm{S}_{mk}^{(jl)}-%
					     (\mathbbm{S}^{(j0)}\mathbbm{S}^{-1}\mathbbm{S}^{(0l)})_{mk}\right)\dot{\lambda}_{kl}$$
$$Y_{m}^j=\sum_{k=1}^N\rho_{mk}\left(\mathbbm{H}_{mk}^{(j0)}-%
	                     (\mathbbm{S}^{(j0)}\mathbbm{S}^{-1}\mathbbm{H})_{mk} \right)$$
$$X_{mk}^{jl}=\rho_{mk}\left(\mathbbm{S}_{mk}^{(jl)}-%
					     (\mathbbm{S}^{(j0)}\mathbbm{S}^{-1}\mathbbm{S}^{(0l)})_{mk}\right)$$
$$i\hbar\dot{\Lambda} = \mathbbm{X}^{-1}\mathbbm{Y},\text{ where }\Lambda\text{ is matrix}$$
Thus, we have two sets of equations:
$$\dot{\vec{C}} = -\frac{i}{\hbar}\mathbbm{S}^{-1}(\mathbbm{H}-i\hbar\tau)\vec{C}$$
$$\dot{\Lambda} = -\frac{i}{\hbar}\mathbbm{X}^{-1}\mathbbm{Y}$$

