First, let's consider time dependent Hellmann--Feynman theorem, 
when $|\Psi\rangle=|g\rangle$ --- one gaussian wave packet, 
$\varepsilon = \vec{q}$ or $\vec{p}$, $\hbar=1$.

$$\left\langle g\left|\frac{\partial\hat{H}}{\partial \vec{q}}\right|g\right\rangle=i\frac{\partial}{\partial t}\left\langle g\left|\frac{\partial g}{\partial \vec{q}}\right.\right\rangle$$
$$\left|\frac{\partial g}{\partial \vec{q}}\right\rangle = (\omega(\vec{r}-\vec{q})-i\vec{p})|g\rangle$$
$$\left\langle g\left|\frac{\partial g}{\partial\vec{q}}\right.\right\rangle = \omega\langle g|\vec{r}|g\rangle - \vec{\xi}\langle g|g\rangle$$
$$\left\langle g\left|\frac{\partial g}{\partial\vec{q}}\right.\right\rangle = \left(\frac{\vec{\xi}^*+\vec{\xi}}{2} -\vec{\xi}\right)\langle g|g\rangle$$
$$\left\langle g\left|\frac{\partial g}{\partial\vec{q}}\right.\right\rangle = \left(\frac{\vec{\xi}^*-\vec{\xi}}{2}\right)\langle g|g\rangle$$
$$\left\langle g\left|\frac{\partial g}{\partial\vec{q}}\right.\right\rangle = \left(\frac{\vec{\xi}^*-\vec{\xi}}{2}\right)\langle g|g\rangle$$
$$\left\langle g\left|\frac{\partial g}{\partial\vec{q}}\right.\right\rangle = -i\vec{p}\langle g|g\rangle$$
$$\left\langle g\left|\frac{\partial\hat{H}}{\partial \vec{q}}\right|g\right\rangle=\frac{\partial}{\partial t} \left(\vec{p}\langle g|g\rangle\right)$$

As norm is conserved, we will obtain:
$$\dot{\vec{p}}=\frac{\left\langle g\left|\frac{\partial\hat{H}}{\partial \vec{q}}\right|g\right\rangle}{\langle g|g\rangle}$$

For parameter $\vec{p}$:
$$\left\langle g\left|\frac{\partial\hat{H}}{\partial \vec{p}}\right|g\right\rangle=i\frac{\partial}{\partial t}\left\langle g\left|\frac{\partial g}{\partial \vec{p}}\right.\right\rangle$$
$$\left|\frac{\partial g}{\partial \vec{p}}\right\rangle = i(\vec{r}-\vec{q})|g\rangle$$
$$\left\langle g\left|\frac{\partial g}{\partial \vec{p}}\right.\right\rangle = i\langle g|(\vec{r}-\vec{q})|g\rangle$$
$$\left\langle g\left|\frac{\partial g}{\partial \vec{p}}\right.\right\rangle = i\langle g|\vec{r}|g\rangle-i\vec{q}\langle g|g\rangle$$
$$\left\langle g\left|\frac{\partial g}{\partial \vec{p}}\right.\right\rangle = 0 $$
$$\left\langle g\left|\frac{\partial\hat{H}}{\partial \vec{p}}\right|g\right\rangle=0$$

Let us consider Hellmann--Feynman equation with repsect to time as $\varepsilon$:
$$\left\langle g\left|\frac{\partial\hat{H}}{\partial t}\right|g\right\rangle=i\frac{\partial}{\partial t}\left\langle g\left|\frac{\partial g}{\partial t}\right.\right\rangle$$
The left side is equal to zero, the right side:
$$\left\langle g\left|\frac{\partial g}{\partial t}\right.\right\rangle = %
  \left\langle g\left|\frac{\partial g}{\partial \vec{q}}\right.\right\rangle\dot{\vec{q}} + %
  \left\langle g\left|\frac{\partial g}{\partial \vec{p}}\right.\right\rangle\dot{\vec{p}}=$$
$$=-i\vec{p}\dot{\vec{q}}\langle g|g\rangle$$
$$\frac{\partial\vec{p}\dot{\vec{q}}}{\partial t}\langle g|g\rangle = 0$$
$$\frac{\partial \vec{p}\dot{\vec{q}}}{\partial t}=0$$

